lemmas about the first switch statement, two cases of the main lemma

src/strtoimax/asn_strtoimax_lim_proof.v
@@ -3,26 +3,29 @@ From compcert Require Import Coqlib Integers Floats AST Ctypes Cop Clight Clight
 Import ListNotations.
 Require Import StructTact.StructTactics.
 Require Import IntNotations asn_strtoimax_lim IntLemmas Tactics asn_strtoimax_lim_spec.
+Require Import switch_statements.
 Local Open Scope Int64Scope.
 
 (* Lemmas for each `asn_strtox_result_e` case *)
 (* Case ASN_STRTOX_ERROR_INVAL: str >= *end *)
 Lemma asn_strtoimax_lim_ASN_STRTOX_ERROR_INVAL_correct : forall le str fin inp m' val ip,
- le ! _str = Some (vptr str) ->
- le ! _end = Some (vptr fin) ->
- le ! _intp = Some (vptr inp) ->
- le ! _upper_boundary = Some (Vlong upper_boundary) ->
- le ! _sign = Some (Vint (Int.repr 1)) ->
- asn_strtoimax_lim str fin inp =
- Some
-   {|
-   return_type := ASN_STRTOX_ERROR_INVAL;
-   value := val;
-   intp := ip;
-   memory := Some m' |} ->
- exists (t : trace) (le' : temp_env),
-   exec_stmt ge e le m (fn_body f_asn_strtoimax_lim) t le' m'
-     (Out_return (Some (Vint (asn_strtox_result_e_to_int ASN_STRTOX_ERROR_INVAL), tint))).
+    le ! _str = Some (vptr str) ->
+    le ! _end = Some (vptr fin) ->
+    le ! _intp = Some (vptr inp) ->
+    le ! _upper_boundary = Some (Vlong upper_boundary) ->
+    le ! _sign = Some (Vint (Int.repr 1)) ->
+    
+    asn_strtoimax_lim str fin inp =
+    Some
+      {|
+        return_type := ASN_STRTOX_ERROR_INVAL;
+        value := val;
+        intp := ip;
+        memory := Some m' |} ->
+    
+    exists (t : trace) (le' : temp_env),
+      exec_stmt ge e le m (fn_body f_asn_strtoimax_lim) t le' m'
+                (Out_return (Some (Vint (asn_strtox_result_e_to_int ASN_STRTOX_ERROR_INVAL), tint))).
 Proof.
   intros until ip; intros Str End Intp UB Sign Spec. unfold vptr in *; repeat break_let; subst; simpl in Spec.                       
   unfold asn_strtoimax_lim in Spec.
@@ -118,7 +121,7 @@ Lemma asn_strtoimax_lim_ASN_STRTOX_EXPECT_MORE_correct : forall le str fin inp m
    exec_stmt ge e le m (fn_body f_asn_strtoimax_lim) t le' m'
      (Out_return (Some (Vint (asn_strtox_result_e_to_int ASN_STRTOX_EXPECT_MORE), tint))).
 Proof.
-  replace (asn_strtox_result_e_to_int ASN_STRTOX_EXPECT_MORE) with (Int.repr (-1)) by (cbv; auto).
+ (* replace (asn_strtox_result_e_to_int ASN_STRTOX_EXPECT_MORE) with (Int.repr (-1)) by (cbv; auto).
   intros until ip; intros Str End Intp UB Sign Spec. unfold vptr in *; repeat break_let; subst; simpl in Spec.    
   assert (forall dist str fin intp v s last_digit  m',
              asn_strtoimax_lim_loop str fin intp v s last_digit dist m <>  Some
@@ -290,308 +293,8 @@ Proof.
 
    pose proof (Loop (distance (b1, i1) (b2, i2) - 1)%nat ((b1, i1) ++) (b0, i0) (b, i) 0 Unsigned last_digit_max). congruence.
  pose proof (Loop (distance (b1, i1) (b2, i2))%nat ((b1, i1)) (b0, i0) (b, i) 0 Unsigned last_digit_max). congruence.
-  Qed.
-
-
-(* Dealing with the switch statement *)
-Definition switch s1 s2 :=  (Sswitch (Ederef (Etempvar _str (tptr tschar)) tschar)
-                      (LScons (Some 48)
-                        Sskip
-                        (LScons (Some 49)
-                          Sskip
-                          (LScons (Some 50)
-                            Sskip
-                            (LScons (Some 51)
-                              Sskip
-                              (LScons (Some 52)
-                                Sskip
-                                (LScons (Some 53)
-                                  Sskip
-                                  (LScons (Some 54)
-                                    Sskip
-                                    (LScons (Some 55)
-                                      Sskip
-                                      (LScons (Some 56)
-                                        Sskip
-                                        (LScons (Some 57)
-                                         s1       
-                                         
-                                          (LScons None
-                                            s2
-                                            LSnil)))))))))))).
-
-(* If reading i a digit then we enter the correct branch and continue *)
-Lemma switch_correct_continue : forall i s1 s2 le b ofs,
-    Mem.loadv Mint8signed m (Vptr b ofs) = Some (Vint i) ->
-    le ! _str = Some (Vptr b ofs) ->
-    is_digit i = true ->
-    forall le', (exists t, exec_stmt ge e le m s1 t le' m Out_continue) ->
-    (exists t, exec_stmt ge e le m (switch s1 s2) t le' m Out_continue).
-Proof.
-  intros.
-  cbn in H1.
-  break_exists.
-  repeat destruct_orb_hyp.
-  11: congruence.
-  all: assert (outcome_switch Out_continue = Out_continue) as Out by (simpl; auto); rewrite <- Out; repeat eexists; try reflexivity; repeat econstructor; try eassumption; try econstructor; (switch_destruct i).
-  1-9: eapply exec_Sseq_1; repeat (choose_seq s1); try (exec_Axiom || eassumption || discriminate).
-   eapply exec_Sseq_2. try (eassumption || econstructor || discriminate).
-   discriminate.
-Qed.
-
-(* If reading i a digit then we enter the correct branch and continue *)
-Lemma switch_default_correct : forall i 
-                       s1 s2 le b ofs out,
-    Mem.loadv Mint8signed m (Vptr b ofs) = Some (Vint i) ->
-    le ! _str = Some (Vptr b ofs) ->
-    is_digit i = false ->
-    forall le' m', (exists t, exec_stmt ge e le m s2 t le' m' (Out_return out)) ->
-                (exists t, exec_stmt ge e le m (switch s1 s2) t le' m' (Out_return out)).
-Proof.
-  intros until out; intros Mem Str Dig le' m' S2.
-  destruct S2 as [t S2].
-  repeat eexists.
-  replace (Out_return out) with (outcome_switch (Out_return out)) by (reflexivity).
-  econstructor.
-  repeat econstructor; try eassumption.
-  econstructor.
-  cbn in Dig.
-  repeat destruct_orb_hyp.
-  repeat (switch_destruct i).
-  try (rewrite Int.unsigned_repr in *).
-  unfold select_switch.
-  unfold select_switch_default.
-  unfold select_switch_case.
-  repeat break_if.
-  all: try congruence.
-  eapply exec_Sseq_2.
-  eassumption.
-  discriminate.
-  all: cbn;  try lia.
-       Qed.
-
-Lemma switch_correct_return : forall i s1 s2 le b ofs out,
-    Mem.loadv Mint8signed m (Vptr b ofs) = Some (Vint i) ->
-    le ! _str = Some (Vptr b ofs) ->
-    is_digit i = true ->
-    forall le' m', (exists t, exec_stmt ge e le m s1 t le' m' (Out_return out)) ->
-    (exists t, exec_stmt ge e le m (switch s1 s2) t le' m' (Out_return out)).
-Proof.
-  intros.
-  cbn in H1.
-  break_exists.
-  repeat destruct_orb_hyp.
-  11: congruence.
-  all: assert (outcome_switch (Out_return out) = (Out_return out)) as Out by (simpl; auto); rewrite <- Out; repeat eexists; try reflexivity; repeat econstructor; try eassumption; try econstructor; (switch_destruct i).
-  1-9: eapply exec_Sseq_1; repeat (choose_seq s1); try (exec_Axiom || eassumption || discriminate).
-   eapply exec_Sseq_2. try (eassumption || econstructor || discriminate).
-   discriminate.
-Qed.
-
-Lemma asn_strtoimax_lim_loop_ASN_STRTOX_ERROR_RANGE_correct : forall dist b ofs le str fin intp inp_value  m' val ip,
-    
-    le!_str = Some (vptr str)  ->
-    le!_end = Some (vptr fin) ->
-    le!_intp = Some (vptr intp)  ->
-    le!_value = Some (Vlong inp_value) ->
-    le ! _upper_boundary = Some (Vlong upper_boundary) ->
-    le ! _sign = Some (Vint (Int.repr 1)) ->
-
-    load_addr Mptr m fin = Some (Vptr b ofs) ->
-
-    (distance str (b,ofs)) = dist ->
-
-    asn_strtoimax_lim_loop str fin intp inp_value Unsigned last_digit_max dist m = Some {| return_type := ASN_STRTOX_ERROR_RANGE;
-              value := val;
-              intp := ip;
-              memory := Some m'; 
-           |}  ->
-
-    exists t le', exec_stmt ge e le m f_asn_strtoimax_lim_loop t le' m' (Out_return (Some (Vint (asn_strtox_result_e_to_int ASN_STRTOX_ERROR_RANGE), tint))).         
-Proof.
-  replace (asn_strtox_result_e_to_int ASN_STRTOX_ERROR_RANGE) with (Int.repr (-3)) by (reflexivity).
-  induction dist; intros until ip; intros Str End Intp Value UB Sign Load Dist Spec;
-    unfold vptr in *; repeat break_let;  simpl in Spec.
-  - break_match. all: congruence.
-  - repeat break_match.
-    all: try congruence.
-    (* 3 cases *)
-     + remember ((_str <~ Vptr b2 (i1 + 1)%ptrofs)
-              ((_value <~ Vlong (inp_value * int_to_int64 (Int.repr 10) + int_to_int64 (i2 - zero_char)%int))
-              ((_d <~ Vint (i2 - zero_char)%int)
-              ((_t'2 <~ Vint i2) ((_t'1 <~ Vint zero_char) ((_t'3 <~ Vptr b ofs) le)))))) as le''.
-     pose proof (IHdist b ofs le'' (b2, (i1 + 1)%ptrofs) (b1, i0) intp 
-           (inp_value * Int64.repr 10 + int_to_int64 (i2 - zero_char)%int)  
-           m' val ip) as IH.
-     clear IHdist.
-     destruct IH as [t IH]; subst; try (repeat env_assumption || reflexivity).
-     admit. (* follows from Dist *)    
-     destruct IH as [le' IH].
-      pose proof (switch_correct_continue i2 switch_body switch_default  (PTree.set _t'1 (Vint i2) (PTree.set _t'3 (Vptr b ofs) le)) b2 i1) as SW.
-      unfold switch in SW.
-      assert (Mem.loadv Mint8signed m (Vptr b2 i1) = Some (Vint i2)) as M by (simpl; eassumption).
-      assert (((_t'1 <~ Vint i2) ((_t'3 <~ Vptr b ofs) le)) ! _str = Some (Vptr b2 i1)) as L by (repeat env_assumption).
-      pose proof (SW M L Heqb3  ((_value <~
-      Vlong
-        (inp_value * cast_int_long Signed (Int.repr 10) +
-         cast_int_long Signed (i2 - zero_char)%int))
-       ((_d <~ Vint (i2 - zero_char)%int)
-          ((_t'2 <~ Vint i2) ((_t'1 <~ Vint zero_char) ((_t'3 <~ Vptr b ofs) le)))))).
-     assert ((exists t : trace,
-         exec_stmt ge e ((_t'1 <~ Vint i2) ((_t'3 <~ Vptr b ofs) le)) m switch_body t
-           ((_value <~
-             Vlong
-               (inp_value * cast_int_long Signed (Int.repr 10) +
-                cast_int_long Signed (i2 - zero_char)%int))
-              ((_d <~ Vint (i2 - zero_char)%int)
-                 ((_t'2 <~ Vint i2) ((_t'1 <~ Vint zero_char) ((_t'3 <~ Vptr b ofs) le)))))
-           m Out_continue)) as F by admit. 
-     pose proof (H F).
-     destruct H0.
-     repeat eexists.
-     eapply exec_Sloop_loop.
-     instantiate (1 := Out_continue).
-     econstructor. (* Wrong local env instantiated  by repeat econstructor ??? *)
-     econstructor.
-     econstructor.
-     repeat econstructor; try env_assumption.
-     repeat econstructor; try env_assumption.
-     try eassumption.
-     econstructor.
-     assert (sem_cmp Clt (Vptr b2 i1) (tptr tschar) (Vptr b ofs) (tptr tschar) m = Some Vtrue) by admit. (* follows from Dist *)
-     eassumption.
-     repeat econstructor.
-     replace (negb (1 == 0)%int) with true by (auto with ints).
-     econstructor.
-     econstructor.
-     repeat econstructor; try env_assumption; try eassumption.
-     simpl.
-     assert (Mem.load Mint8signed m b2 (Ptrofs.unsigned i1) = Some (Vint i2)) by  (simpl; eassumption). 
-     eassumption.
-     econstructor.
-     repeat econstructor.
-     repeat env_assumption.
-     repeat econstructor.
-     fold f_asn_strtoimax_lim_loop.
-     replace  (i0 + Ptrofs.repr (sizeof ge tschar) * ptrofs_of_int Signed (Int.repr 1))%ptrofs with (i0 + 1)%ptrofs.
-     replace (inp_value * cast_int_long Signed (Int.repr 10) +
-            cast_int_long Signed (i2 - zero_char)%int) with  (inp_value * int_to_int64 (Int.repr 10) +
-                                                              int_to_int64 (i2 - zero_char)%int).
-     
-     eapply IH.
-     simpl.
-     unfold int_to_int64.
-     admit. (* signed and unsigned ? *)
-     auto with ptrofs.
-     +
-
-   remember ((_str <~ Vptr b2 (i1 + 1)%ptrofs)
-              ((_value <~ Vlong (inp_value * int_to_int64 (Int.repr 10) + int_to_int64 (i2 - zero_char)%int))
-              ((_d <~ Vint (i2 - zero_char)%int)
-              ((_t'2 <~ Vint i2) ((_t'1 <~ Vint zero_char) ((_t'3 <~ Vptr b ofs) le)))))) as le''.
-     pose proof (IHdist b ofs le'' (b2, (i1 + 1)%ptrofs) (b1, i0) intp 
-           (inp_value * Int64.repr 10 + int_to_int64 (i2 - zero_char)%int)  
-           m' val ip) as IH.
-     clear IHdist.
-     destruct IH as [t IH]; subst; try (repeat env_assumption || reflexivity).
-     admit. (* follows from Dist *)    
-     destruct IH as [le' IH].
-      pose proof (switch_correct_continue i2 switch_body switch_default  (PTree.set _t'1 (Vint i2) (PTree.set _t'3 (Vptr b ofs) le)) b2 i1) as SW.
-      unfold switch in SW.
-      assert (Mem.loadv Mint8signed m (Vptr b2 i1) = Some (Vint i2)) as M by (simpl; eassumption).
-      assert (((_t'1 <~ Vint i2) ((_t'3 <~ Vptr b ofs) le)) ! _str = Some (Vptr b2 i1)) as L by (repeat env_assumption).
-      pose proof (SW M L Heqb3  ((_value <~
-      Vlong
-        (inp_value * cast_int_long Signed (Int.repr 10) +
-         cast_int_long Signed (i2 - zero_char)%int))
-       ((_d <~ Vint (i2 - zero_char)%int)
-          ((_t'2 <~ Vint i2) ((_t'1 <~ Vint zero_char) ((_t'3 <~ Vptr b ofs) le)))))).
-     assert ((exists t : trace,
-         exec_stmt ge e ((_t'1 <~ Vint i2) ((_t'3 <~ Vptr b ofs) le)) m switch_body t
-           ((_value <~
-             Vlong
-               (inp_value * cast_int_long Signed (Int.repr 10) +
-                cast_int_long Signed (i2 - zero_char)%int))
-              ((_d <~ Vint (i2 - zero_char)%int)
-                 ((_t'2 <~ Vint i2) ((_t'1 <~ Vint zero_char) ((_t'3 <~ Vptr b ofs) le)))))
-           m Out_continue)) as F by admit. 
-     pose proof (H F).
-     destruct H0.
-     repeat eexists.
-     eapply exec_Sloop_loop.
-     instantiate (1 := Out_continue).
-     econstructor. (* Wrong local env instantiated  by repeat econstructor ??? *)
-     econstructor.
-     econstructor.
-     repeat econstructor; try env_assumption.
-     repeat econstructor; try env_assumption.
-     try eassumption.
-     econstructor.
-     assert (sem_cmp Clt (Vptr b2 i1) (tptr tschar) (Vptr b ofs) (tptr tschar) m = Some Vtrue) by admit. (* follows from Dist *)
-     eassumption.
-     repeat econstructor.
-     replace (negb (1 == 0)%int) with true by (auto with ints).
-     econstructor.
-     econstructor.
-     repeat econstructor; try env_assumption; try eassumption.
-     simpl.
-     assert (Mem.load Mint8signed m b2 (Ptrofs.unsigned i1) = Some (Vint i2)) by  (simpl; eassumption). 
-     eassumption.
-     econstructor.
-     repeat econstructor.
-     repeat env_assumption.
-     repeat econstructor.
-     fold f_asn_strtoimax_lim_loop.
-     replace  (i0 + Ptrofs.repr (sizeof ge tschar) * ptrofs_of_int Signed (Int.repr 1))%ptrofs with (i0 + 1)%ptrofs.
-     replace (inp_value * cast_int_long Signed (Int.repr 10) +
-            cast_int_long Signed (i2 - zero_char)%int) with  (inp_value * int_to_int64 (Int.repr 10) +
-                                                              int_to_int64 (i2 - zero_char)%int).
-     
-     eapply IH.
-     simpl.
-     unfold int_to_int64.
-     admit. (* signed and unsigned ? *)
-     auto with ptrofs.
-
-    + inversion Spec.
-      unfold  Mem.loadv in *.
-      assert (((_t'1 <~ Vint i2) ((_t'3 <~ Vptr b ofs) le)) ! _str = Some (Vptr b2 i1)) as LE by (repeat env_assumption).
-      assert (Mem.loadv Mint8signed asn_strtoimax_lim_spec.m (Vptr b2 i1) = Some (Vint i2)) as M by (simpl; eassumption).
-      assert (((_t'1 <~ Vint i2) ((_t'3 <~ Vptr b ofs) le)) ! _str = Some (Vptr b2 i1)) as L by (repeat env_assumption).
-      pose proof (switch_correct_return i2 switch_body switch_default  (PTree.set _t'1 (Vint i2) (PTree.set _t'3 (Vptr b ofs) le))  b2 i1 ((Some (Vint (Int.repr (-3)), tint)))) as SW.
-     
-     pose proof (SW M L Heqb3  ((_value <~
-      Vlong
-        (inp_value * cast_int_long Signed (Int.repr 10) +
-         cast_int_long Signed (i2 - zero_char)%int))
-       ((_d <~ Vint (i2 - zero_char)%int)
-          ((_t'2 <~ Vint i2) ((_t'1 <~ Vint i2) ((_t'3 <~ Vptr b ofs) le))))) m).
-     
-       destruct H.
-      ++ admit. 
-      ++
-        repeat eexists.
-        eapply exec_Sloop_stop1.
-        econstructor. (* Wrong local env instantiated  by repeat econstructor ??? *)
-        econstructor.
-        econstructor.
-        repeat econstructor; try env_assumption.
-        repeat econstructor; try env_assumption.
-        try eassumption.
-        econstructor.
-        simpl.
-        assert (sem_cmp Clt (Vptr b2 i1) (tptr tschar) (Vptr b ofs) (tptr tschar) asn_strtoimax_lim_spec.m = Some Vtrue) by admit. eassumption.
-        econstructor.
-        econstructor.
-        econstructor.
-        repeat econstructor.
-        1-2: env_assumption.
-        env_assumption.
-        replace m' with m by auto.
-        unfold switch in H.
-        eassumption.
-        econstructor.
-Admitted.
+  Qed. *)
+  Admitted.
 
 (* Loop correctness cases *)
 (* ASN_STRTOX_OK: conversion successfull *)
@@ -617,12 +320,11 @@ Lemma asn_strtoimax_lim_loop_ASN_STRTOX_OK_correct :  forall dist b ofs le str f
 
     exists t le', exec_stmt ge e le m f_asn_strtoimax_lim_loop t le' m' (Out_return (Some (Vint (asn_strtox_result_e_to_int ASN_STRTOX_OK), tint))). 
  Proof.
-   (* induction dist; intros until m'; intros Str End Value UB LastD Sign Load Dist Spec; unfold vptr in *; repeat break_let; subst; simpl in Spec.
+  (*  induction dist; intros until ip; intros Str End Value UB LastD Sign Load Dist Spec; unfold vptr in *; repeat break_let; subst; simpl in Spec.
    - (* Base case *)
      
      break_match.
      inversion Spec.
-     rewrite <- H0.
      repeat eexists.
      eapply exec_Sloop_stop1.
      eapply exec_Sseq_2.
@@ -825,8 +527,7 @@ Lemma asn_strtoimax_lim_loop_ASN_STRTOX_OK_correct :  forall dist b ofs le str f
      Admitted.
 
  (* Case ASN_STRTOX_EXTRA_DATA: go through the loop until a non-digit encountered *)
-
-   Lemma asn_strtoimax_lim_loop_ASN_STRTOX_EXTRA_DATA_correct : forall dist b ofs le str fin intp inp_value  m' val ip,
+Lemma asn_strtoimax_lim_loop_ASN_STRTOX_EXTRA_DATA_correct : forall dist b ofs le str fin intp inp_value  m' val ip,
     
     le!_str = Some (vptr str)  ->
     le!_end = Some (vptr fin) ->
@@ -965,32 +666,225 @@ Proof.
          
 Admitted.
 
-(* Lemma pre_loop_execution : forall s1 s2,
-    le!_str = Some (vptr str)  ->
-    le!_end = Some (vptr fin) ->
-    le!_intp = Some (vptr intp)  ->
-    le ! _upper_boundary = Some (Vlong upper_boundary) ->
-    le ! _sign = Some (Vint (Int.repr 1)) ->
+Definition Sign s :=
+  match s with
+  | Signed => Int.neg (Int.repr 1)
+  | Unsigned => Int.repr 1
+  end.
 
-    asn_strtoimax_lim str fin intp
-    = Some {| return_type := res;
+Lemma asn_strtoimax_lim_loop_ASN_STRTOX_ERROR_RANGE_correct : forall dist b ofs le str_b str_ofs fin_b fin_ofs intp_b intp_ofs inp_value  m' val s ip,
+    
+    le!_str = Some (Vptr str_b str_ofs)  ->
+    le!_end = Some (Vptr fin_b fin_ofs) ->
+    le!_intp = Some (Vptr intp_b intp_ofs)  ->
+    le!_value = Some (Vlong inp_value) ->
+    le ! _upper_boundary = Some (Vlong upper_boundary) ->
+    le ! _sign = Some (Vint (Sign s)) ->
+
+    load_addr Mptr m (fin_b, fin_ofs) = Some (Vptr b ofs) ->
+
+    (distance (str_b, str_ofs) (b,ofs)) = dist ->
+
+    asn_strtoimax_lim_loop (str_b, str_ofs) (fin_b, fin_ofs) (intp_b, intp_ofs) inp_value s (max_sign s) dist m = Some {| return_type := ASN_STRTOX_ERROR_RANGE;
               value := val;
               intp := ip;
               memory := Some m'; 
-           |} ->
+           |}  ->
 
-    forall le' m', (exists t , exec_stmt ge e le m (pre_loop s1 s2) t le' m' Out_return ->
-    exists t le', exec_stmt ge e le m (pre_loop s1 s2) t le' m' out. *)
+    exists t le', exec_stmt ge e le m f_asn_strtoimax_lim_loop t le' m' (Out_return (Some (Vint (asn_strtox_result_e_to_int ASN_STRTOX_ERROR_RANGE), tint))).         
+Proof.
+  replace (asn_strtox_result_e_to_int ASN_STRTOX_ERROR_RANGE) with (Int.repr (-3)) by (reflexivity).
+  induction dist; intros until ip; intros Str End Intp Value UB Sign Load Dist Spec;
+    unfold vptr in *; repeat break_let;  simpl in Spec.
+  - break_match. all: congruence.
+  - repeat break_match.
+    all: try congruence.
+    (* 3 cases *)
+     + remember ((_str <~ Vptr str_b (str_ofs + 1)%ptrofs)
+              ((_value <~ Vlong (inp_value * int_to_int64 (Int.repr 10) + int_to_int64 (i - zero_char)%int))
+              ((_d <~ Vint (i - zero_char)%int)
+              ((_t'2 <~ Vint i) ((_t'1 <~ Vint zero_char) ((_t'3 <~ Vptr b ofs) le)))))) as le''.
+     pose proof (IHdist b ofs le'' str_b (str_ofs + 1)%ptrofs fin_b fin_ofs intp_b intp_ofs 
+           (inp_value * Int64.repr 10 + int_to_int64 (i - zero_char)%int)  
+           m' val s ip) as IH.
+     clear IHdist.
+     destruct IH as [t IH]; subst; try (repeat env_assumption || reflexivity).
+     admit. (* follows from Dist *)    
+     destruct IH as [le' IH].
+     pose proof (switch_correct_continue i switch_body switch_default (PTree.set _t'1 (Vint i) (PTree.set _t'3 (Vptr b ofs) le))  str_b str_ofs) as SW.
+      unfold switch in SW.
+      assert (Mem.loadv Mint8signed m (Vptr str_b str_ofs) = Some (Vint i)) as M by (simpl; eassumption).
+      assert (((_t'1 <~ Vint i) ((_t'3 <~ Vptr b ofs) le)) ! _str = Some (Vptr str_b str_ofs)) as L by (repeat env_assumption).
+      pose proof (SW M L Heqb0  ((_value <~
+      Vlong
+        (inp_value * cast_int_long Signed (Int.repr 10) +
+         cast_int_long Signed (i - zero_char)%int))
+       ((_d <~ Vint (i - zero_char)%int)
+          ((_t'2 <~ Vint i) ((_t'1 <~ Vint zero_char) ((_t'3 <~ Vptr b ofs) le)))))).
+     assert ((exists t : trace,
+         exec_stmt ge e ((_t'1 <~ Vint i) ((_t'3 <~ Vptr b ofs) le)) m switch_body t
+           ((_value <~
+             Vlong
+               (inp_value * cast_int_long Signed (Int.repr 10) +
+                cast_int_long Signed (i - zero_char)%int))
+              ((_d <~ Vint (i - zero_char)%int)
+                 ((_t'2 <~ Vint i) ((_t'1 <~ Vint zero_char) ((_t'3 <~ Vptr b ofs) le)))))
+           m Out_continue)) as F by admit. 
+     pose proof (H F).
+     destruct H0.
+     repeat eexists.
+     eapply exec_Sloop_loop.
+     instantiate (1 := Out_continue).
+     econstructor. (* Wrong local env instantiated  by repeat econstructor ??? *)
+     econstructor.
+     econstructor.
+     repeat econstructor; try env_assumption.
+     repeat econstructor; try env_assumption.
+     try eassumption.
+     econstructor.
+     assert (sem_cmp Clt (Vptr str_b str_ofs) (tptr tschar) (Vptr b ofs) (tptr tschar) m = Some Vtrue) by admit. (* follows from Dist *)
+     eassumption.
+     repeat econstructor.
+     replace (negb (1 == 0)%int) with true by (auto with ints).
+     econstructor.
+     econstructor.
+     repeat econstructor; try env_assumption; try eassumption.
+     eassumption.
+     econstructor.
+     econstructor.
+     repeat econstructor.
+     repeat env_assumption.
+     repeat econstructor.
+     fold f_asn_strtoimax_lim_loop.
+     replace  (str_ofs + Ptrofs.repr (sizeof ge tschar) * ptrofs_of_int Signed (Int.repr 1))%ptrofs with (str_ofs + 1)%ptrofs.
+     replace (inp_value * cast_int_long Signed (Int.repr 10) +
+            cast_int_long Signed (i - zero_char)%int) with  (inp_value * int_to_int64 (Int.repr 10) +
+                                                              int_to_int64 (i - zero_char)%int).
+     
+     eapply IH.
+     simpl.
+     unfold int_to_int64.
+     admit. (* signed and unsigned ? *)
+     auto with ptrofs.
+  (*   +
 
-Lemma asn_strtoimax_lim_correct : forall le str fin intp m' res val ip,
+   remember ((_str <~ Vptr str_b (str_ofs + 1)%ptrofs)
+              ((_value <~ Vlong (inp_value * int_to_int64 (Int.repr 10) + int_to_int64 (i - zero_char)%int))
+              ((_d <~ Vint (i - zero_char)%int)
+              ((_t'2 <~ Vint i) ((_t'1 <~ Vint zero_char) ((_t'3 <~ Vptr b ofs) le)))))) as le''.
+     pose proof (IHdist b ofs le'' (str_b, (str_ofs + 1)%ptrofs) (b1, i0) intp 
+           (inp_value * Int64.repr 10 + int_to_int64 (i - zero_char)%int)  
+           m' val s ip) as IH.
+     clear IHdist.
+     destruct IH as [t IH]; subst; try (repeat env_assumption || reflexivity).
+     admit. (* follows from Dist *)    
+     destruct IH as [le' IH].
+      pose proof (switch_correct_continue i switch_body switch_default  (PTree.set _t'1 (Vint i) (PTree.set _t'3 (Vptr b ofs) le)) str_b str_ofs) as SW.
+      unfold switch in SW.
+      assert (Mem.loadv Mint8signed m (Vptr str_b str_ofs) = Some (Vint i)) as M by (simpl; eassumption).
+      assert (((_t'1 <~ Vint i) ((_t'3 <~ Vptr b ofs) le)) ! _str = Some (Vptr str_b str_ofs)) as L by (repeat env_assumption).
+      pose proof (SW M L Heqb3  ((_value <~
+      Vlong
+        (inp_value * cast_int_long Signed (Int.repr 10) +
+         cast_int_long Signed (i - zero_char)%int))
+       ((_d <~ Vint (i - zero_char)%int)
+          ((_t'2 <~ Vint i) ((_t'1 <~ Vint zero_char) ((_t'3 <~ Vptr b ofs) le)))))).
+     assert ((exists t : trace,
+         exec_stmt ge e ((_t'1 <~ Vint i) ((_t'3 <~ Vptr b ofs) le)) m switch_body t
+           ((_value <~
+             Vlong
+               (inp_value * cast_int_long Signed (Int.repr 10) +
+                cast_int_long Signed (i - zero_char)%int))
+              ((_d <~ Vint (i - zero_char)%int)
+                 ((_t'2 <~ Vint i) ((_t'1 <~ Vint zero_char) ((_t'3 <~ Vptr b ofs) le)))))
+           m Out_continue)) as F by admit. 
+     pose proof (H F).
+     destruct H0.
+     repeat eexists.
+     eapply exec_Sloop_loop.
+     instantiate (1 := Out_continue).
+     econstructor. (* Wrong local env instantiated  by repeat econstructor ??? *)
+     econstructor.
+     econstructor.
+     repeat econstructor; try env_assumption.
+     repeat econstructor; try env_assumption.
+     try eassumption.
+     econstructor.
+     assert (sem_cmp Clt (Vptr str_b str_ofs) (tptr tschar) (Vptr b ofs) (tptr tschar) m = Some Vtrue) by admit. (* follows from Dist *)
+     eassumption.
+     repeat econstructor.
+     replace (negb (1 == 0)%int) with true by (auto with ints).
+     econstructor.
+     econstructor.
+     repeat econstructor; try env_assumption; try eassumption.
+     simpl.
+     assert (Mem.load Mint8signed m str_b (Ptrofs.unsigned str_ofs) = Some (Vint i)) by  (simpl; eassumption). 
+     eassumption.
+     econstructor.
+     repeat econstructor.
+     repeat env_assumption.
+     repeat econstructor.
+     fold f_asn_strtoimax_lim_loop.
+     replace  (i0 + Ptrofs.repr (sizeof ge tschar) * ptrofs_of_int Signed (Int.repr 1))%ptrofs with (i0 + 1)%ptrofs.
+     replace (inp_value * cast_int_long Signed (Int.repr 10) +
+            cast_int_long Signed (i - zero_char)%int) with  (inp_value * int_to_int64 (Int.repr 10) +
+                                                              int_to_int64 (i - zero_char)%int).
+     
+     eapply IH.
+     simpl.
+     unfold int_to_int64.
+     admit. (* signed and unsigned ? *)
+     auto with ptrofs.
+
+    + inversion Spec.
+      unfold  Mem.loadv in *.
+      assert (((_t'1 <~ Vint i) ((_t'3 <~ Vptr b ofs) le)) ! _str = Some (Vptr str_b str_ofs)) as LE by (repeat env_assumption).
+      assert (Mem.loadv Mint8signed asn_strtoimax_lim_spec.m (Vptr str_b str_ofs) = Some (Vint i)) as M by (simpl; eassumption).
+      assert (((_t'1 <~ Vint i) ((_t'3 <~ Vptr b ofs) le)) ! _str = Some (Vptr str_b str_ofs)) as L by (repeat env_assumption).
+      pose proof (switch_correct_return i switch_body switch_default  (PTree.set _t'1 (Vint i) (PTree.set _t'3 (Vptr b ofs) le))  str_b str_ofs ((Some (Vint (Int.repr (-3)), tint)))) as SW.
+     
+     pose proof (SW M L Heqb3  ((_value <~
+      Vlong
+        (inp_value * cast_int_long Signed (Int.repr 10) +
+         cast_int_long Signed (i - zero_char)%int))
+       ((_d <~ Vint (i - zero_char)%int)
+          ((_t'2 <~ Vint i) ((_t'1 <~ Vint i) ((_t'3 <~ Vptr b ofs) le))))) m).
+     
+       destruct H.
+      ++ admit. 
+      ++
+        repeat eexists.
+        eapply exec_Sloop_stop1.
+        econstructor. (* Wrong local env instantiated  by repeat econstructor ??? *)
+        econstructor.
+        econstructor.
+        repeat econstructor; try env_assumption.
+        repeat econstructor; try env_assumption.
+        try eassumption.
+        econstructor.
+        simpl.
+        assert (sem_cmp Clt (Vptr str_b str_ofs) (tptr tschar) (Vptr b ofs) (tptr tschar) asn_strtoimax_lim_spec.m = Some Vtrue) by admit. eassumption.
+        econstructor.
+        econstructor.
+        econstructor.
+        repeat econstructor.
+        1-2: env_assumption.
+        env_assumption.
+        replace m' with m by auto.
+        unfold switch in H.
+        eassumption.
+        econstructor. *)
+Admitted.
+
+Lemma asn_strtoimax_lim_correct : forall le str_b str_ofs fin_b fin_ofs intp_b intp_ofs m' res val ip,
     
-    le!_str = Some (vptr str)  ->
-    le!_end = Some (vptr fin) ->
-    le!_intp = Some (vptr intp)  ->
+    le!_str = Some (Vptr str_b str_ofs)  ->
+    le!_end = Some (Vptr fin_b fin_ofs) ->
+    le!_intp = Some (Vptr intp_b intp_ofs)  ->
     le ! _upper_boundary = Some (Vlong upper_boundary) ->
     le ! _sign = Some (Vint (Int.repr 1)) ->
 
-    asn_strtoimax_lim str fin intp
+    asn_strtoimax_lim (str_b, str_ofs) (fin_b,fin_ofs) (intp_b,intp_ofs)
     = Some {| return_type := res;
               value := val;
               intp := ip;
@@ -999,291 +893,42 @@ Lemma asn_strtoimax_lim_correct : forall le str fin intp m' res val ip,
     exists t le', exec_stmt ge e le m f_asn_strtoimax_lim.(fn_body) t le' m'
                  (Out_return (Some ((Vint (asn_strtox_result_e_to_int res)), tint))).
 Proof.
-  induction res.
-  - (* ASN_STRTOX_ERROR_RANGE *)
-    intros until ip; intros Str End Intp UB Sign Spec. unfold vptr in *; repeat break_let; subst; simpl in Spec.
-    unfold asn_strtoimax_lim in Spec.
-    repeat break_match.
-    all: try congruence.
-     assert (exists t2 le',  exec_stmt ge e
-    ((_value <~ Vlong (cast_int_long Signed (Int.repr 0)))
-       ((_t'5 <~ Vptr b2 i2)
-          ((_str <~
-            Vptr b1
-              (i1 + Ptrofs.repr (sizeof ge tschar) * ptrofs_of_int Signed (Int.repr 1))%ptrofs)
-             ((_sign <~ Vint (Int.neg (Int.repr 1)))
-                ((_last_digit_max <~
-                  Vlong
-                    (Int64.modu
-                       (Int64.not (cast_int_long Signed (Int.repr 0)) >>
-                        Int64.repr (Int.unsigned (Int.repr 1)))
-                       (cast_int_long Signed (Int.repr 10)) +
-                     cast_int_long Signed (Int.repr 1)))
-                   ((_t'4 <~ Vint minus_char)
-                      ((_t'6 <~ Vptr b2 i2)
-                         ((_last_digit_max <~
-                           Vlong
-                             (Int64.modu
-                                (Int64.not (cast_int_long Signed (Int.repr 0)) >>
-                                 Int64.repr (Int.unsigned (Int.repr 1)))
-                                (cast_int_long Signed (Int.repr 10))))
-                            ((_upper_boundary <~
-                              Vlong
-                                (Int64.divu
-                                   (Int64.not (cast_int_long Signed (Int.repr 0)) >>
-                                    Int64.repr (Int.unsigned (Int.repr 1)))
-                                   (cast_int_long Signed (Int.repr 10))))
-                               ((_sign <~ Vint (Int.repr 1)) le)))))))))) m
-    f_asn_strtoimax_lim_loop t2 le' m'
-    (Out_return (Some (Vint (asn_strtox_result_e_to_int ASN_STRTOX_ERROR_RANGE), tint)))).
-  
-  eapply (asn_strtoimax_lim_loop_ASN_STRTOX_ERROR_RANGE_correct)
-
-  with (le :=  ((_value <~ Vlong (cast_int_long Signed (Int.repr 0)))
-       ((_t'5 <~ Vptr b2 i2)
-          ((_str <~
-            Vptr b1
-              (i1 + Ptrofs.repr (sizeof ge tschar) * ptrofs_of_int Signed (Int.repr 1))%ptrofs)
-             ((_sign <~ Vint (Int.neg (Int.repr 1)))
-                ((_last_digit_max <~
-                  Vlong
-                    (Int64.modu
-                       (Int64.not (cast_int_long Signed (Int.repr 0)) >>
-                        Int64.repr (Int.unsigned (Int.repr 1)))
-                       (cast_int_long Signed (Int.repr 10)) +
-                     cast_int_long Signed (Int.repr 1)))
-                   ((_t'4 <~ Vint minus_char)
-                      ((_t'6 <~ Vptr b2 i2)
-                         ((_last_digit_max <~
-                           Vlong
-                             (Int64.modu
-                                (Int64.not (cast_int_long Signed (Int.repr 0)) >>
-                                 Int64.repr (Int.unsigned (Int.repr 1)))
-                                (cast_int_long Signed (Int.repr 10))))
-                            ((_upper_boundary <~
-                              Vlong
-                                (Int64.divu
-                                   (Int64.not (cast_int_long Signed (Int.repr 0)) >>
-                                    Int64.repr (Int.unsigned (Int.repr 1)))
-                                   (cast_int_long Signed (Int.repr 10))))
-                               ((_sign <~ Vint (Int.repr 1)) le))))))))))) (m' := m').
-  all: repeat env_assumption.
-  1-8:admit.
-  break_exists.
-   
-    repeat eexists.
-    (* case reading minus *)
-   exec_until_seq.
-   econstructor.
-   repeat econstructor.
-   econstructor.
-   repeat econstructor.
-   econstructor.
-   repeat econstructor.
-   repeat env_assumption.
-   eassumption.
-   all: repeat env_assumption.
-   econstructor.
-  
-  simpl in Heqo0.
-  unfold  addr_ge in *.
-  break_let.
-  eapply (ptr_ge_false _ _ _ _  Heqo0).
-  repeat econstructor.
-  repeat econstructor.
-  econstructor.
-  forward.
-  replace  (Out_normal) with (outcome_switch  (Out_normal)).
-  econstructor.
-  forward.
-  forward.
-  replace i3 with minus_char.
-  econstructor.
-  econstructor.
-    exec_until_seq.
-  (rewrite PTree.gso).
-  (rewrite PTree.gso).
-  apply PTree.gss.
-  1-2: cbv; try congruence.
-  1-2: 
-    repeat econstructor.
-  eapply exec_Sseq_1.
-  econstructor.
-  repeat econstructor.
-  all: repeat  env_assumption.
-  unfold tlong.
-  unfold tint.
-  simpl.
-  econstructor.
-  repeat econstructor.
-  all: repeat  env_assumption.
-  repeat econstructor.
-    repeat econstructor.
-  simpl.
-  replace (Ptrofs.repr 1 * Ptrofs.of_ints (Int.repr 1))%ptrofs with (Ptrofs.repr 1) by (auto with ptrofs).
-  assert (sem_cmp Cge (Vptr b1 (i1 + Ptrofs.repr 1)%ptrofs) (tptr tschar) 
-                  (Vptr b2 i2) (tptr tschar) m = Some Vfalse) by admit.
-  eassumption.
-  (* use addr instead of ptr_ge 
-  unfold  addr_ge in *.
-  break_let.
-  pose (ptr_ge_false _ _ _ _ Heqo2).
-  simpl in Heqp.
-  inversion Heqp; subst. *)
-  repeat econstructor.
-  repeat econstructor.
-  econstructor.
-  symmetry.
-  pose (Int.eq_spec i3 minus_char).
-  
-  rewrite Heqb0 in y.
-  auto.
-  simpl.
-  auto.
-  fold f_asn_strtoimax_lim_loop.
-  eapply exec_Sseq_2.
-  econstructor.
-  repeat econstructor.
-  eassumption.
-  congruence.
-
-  (* reading + *)
-
-     assert (exists t2 le',  exec_stmt ge e
-    ((_value <~ Vlong (cast_int_long Signed (Int.repr 0)))
-       ((_t'5 <~ Vptr b2 i2)
-          ((_str <~
-            Vptr b1
-              (i1 + Ptrofs.repr (sizeof ge tschar) * ptrofs_of_int Signed (Int.repr 1))%ptrofs)
-             ((_sign <~ Vint (Int.neg (Int.repr 1)))
-                ((_last_digit_max <~
-                  Vlong
-                    (Int64.modu
-                       (Int64.not (cast_int_long Signed (Int.repr 0)) >>
-                        Int64.repr (Int.unsigned (Int.repr 1)))
-                       (cast_int_long Signed (Int.repr 10)) +
-                     cast_int_long Signed (Int.repr 1)))
-                   ((_t'4 <~ Vint plus_char)
-                      ((_t'6 <~ Vptr b2 i2)
-                         ((_last_digit_max <~
-                           Vlong
-                             (Int64.modu
-                                (Int64.not (cast_int_long Signed (Int.repr 0)) >>
-                                 Int64.repr (Int.unsigned (Int.repr 1)))
-                                (cast_int_long Signed (Int.repr 10))))
-                            ((_upper_boundary <~
-                              Vlong
-                                (Int64.divu
-                                   (Int64.not (cast_int_long Signed (Int.repr 0)) >>
-                                    Int64.repr (Int.unsigned (Int.repr 1)))
-                                   (cast_int_long Signed (Int.repr 10))))
-                               ((_sign <~ Vint (Int.repr 1)) le)))))))))) m
-    f_asn_strtoimax_lim_loop t2 le' m'
-    (Out_return (Some (Vint (asn_strtox_result_e_to_int ASN_STRTOX_ERROR_RANGE), tint)))).
-  
-  eapply (asn_strtoimax_lim_loop_ASN_STRTOX_ERROR_RANGE_correct)
-
-  with (le :=  ((_value <~ Vlong (cast_int_long Signed (Int.repr 0)))
-       ((_t'5 <~ Vptr b2 i2)
-          ((_str <~
-            Vptr b1
-              (i1 + Ptrofs.repr (sizeof ge tschar) * ptrofs_of_int Signed (Int.repr 1))%ptrofs)
-             ((_sign <~ Vint (Int.neg (Int.repr 1)))
-                ((_last_digit_max <~
-                  Vlong
-                    (Int64.modu
-                       (Int64.not (cast_int_long Signed (Int.repr 0)) >>
-                        Int64.repr (Int.unsigned (Int.repr 1)))
-                       (cast_int_long Signed (Int.repr 10)) +
-                     cast_int_long Signed (Int.repr 1)))
-                   ((_t'4 <~ Vint plus_char)
-                      ((_t'6 <~ Vptr b2 i2)
-                         ((_last_digit_max <~
-                           Vlong
-                             (Int64.modu
-                                (Int64.not (cast_int_long Signed (Int.repr 0)) >>
-                                 Int64.repr (Int.unsigned (Int.repr 1)))
-                                (cast_int_long Signed (Int.repr 10))))
-                            ((_upper_boundary <~
-                              Vlong
-                                (Int64.divu
-                                   (Int64.not (cast_int_long Signed (Int.repr 0)) >>
-                                    Int64.repr (Int.unsigned (Int.repr 1)))
-                                   (cast_int_long Signed (Int.repr 10))))
-                               ((_sign <~ Vint (Int.repr 1)) le))))))))))) (m' := m').
-  all: repeat env_assumption.
-  1-7:admit.
-  break_exists.
-   
-    repeat eexists.
-    (* case reading minus *)
-   exec_until_seq.
-   econstructor.
-   repeat econstructor.
-   econstructor.
-   repeat econstructor.
-   econstructor.
-   repeat econstructor.
-   repeat env_assumption.
-   eassumption.
-   all: repeat env_assumption.
-   econstructor.
-  
-  simpl in Heqo0.
-  unfold  addr_ge in *.
-  eapply (ptr_ge_false _ _ _ _  Heqo0).
-  repeat econstructor.
-  repeat econstructor.
-  econstructor.
-  forward.
-  replace  (Out_normal) with (outcome_switch  (Out_normal)).
-  econstructor.
-  forward.
-  forward.
-  replace i3 with plus_char.
-  econstructor.
-  econstructor.
-  exec_until_seq.
-  repeat env_assumption.
-  econstructor.
-  eapply exec_Sseq_1.
-  econstructor.
-  repeat econstructor.
-  all: repeat  env_assumption.
-    repeat econstructor.
-    all: repeat  env_assumption.
-    econstructor.
-    repeat econstructor.
-  unfold tlong.
-  unfold tint.
-  simpl.
-  replace (Ptrofs.repr 1 * Ptrofs.of_ints (Int.repr 1))%ptrofs with (Ptrofs.repr 1) by (auto with ptrofs).
-  assert (sem_cmp Cge (Vptr b1 (i1 + Ptrofs.repr 1)%ptrofs) (tptr tschar) 
-                  (Vptr b2 i2) (tptr tschar) m = Some Vfalse) by admit.
-  eassumption.
-  (* use addr instead of ptr_ge 
-  unfold  addr_ge in *.
-  break_let.
-  pose (ptr_ge_false _ _ _ _ Heqo2).
-  simpl in Heqp.
-  inversion Heqp; subst. *)
-  repeat econstructor.
-  repeat econstructor.
-  econstructor.
-  symmetry.
-  pose (Int.eq_spec i3 plus_char).
-  
-  rewrite Heqb1 in y.
-  auto.
-  simpl.
-  auto.
-  fold f_asn_strtoimax_lim_loop.
-  eapply exec_Sseq_2.
-  econstructor.
-  repeat econstructor.
-  admit.
-  congruence.
-    admit. (* reading no sign *)
+   induction res.
+   - (* ASN_STRTOX_ERROR_RANGE *)
+     intros until ip; intros Str End Intp UB Sign Spec.
+     unfold vptr in *;
+       repeat break_let; subst; simpl in Spec.
+     unfold asn_strtoimax_lim in Spec.
+     repeat break_match.
+     all: try congruence.
+     + destruct_orb_hyp.
+       ++ eapply exec_loop_minus.
+          all: try eassumption.
+          eapply asn_strtoimax_lim_loop_ASN_STRTOX_ERROR_RANGE_correct.
+          1-5: repeat env_assumption; econstructor.
+          instantiate (1 := Signed).
+          all: repeat env_assumption.
+          simpl.
+          econstructor.
+          instantiate (1 := (distance (str_b, str_ofs) (b, i) - 1)%nat).
+          admit. (* distance lemma *)
+          simpl in Spec.
+          switch_destruct i0.
+          rewrite EQ in *.
+          eassumption.     
+       ++ eapply exec_loop_plus.
+          all: try eassumption.
+          eapply asn_strtoimax_lim_loop_ASN_STRTOX_ERROR_RANGE_correct.
+          1-5: repeat env_assumption; econstructor.
+          all: repeat env_assumption.
+          repeat econstructor.
+          switch_destruct i0.
+          unfold sign.
+          break_if; simpl.
+          admit. (* contradiction *)
+          econstructor.
+          admit. (* lemma *)
+      + admit. 
   - eapply asn_strtoimax_lim_ASN_STRTOX_ERROR_INVAL_correct. (* ASN_STRTOX_ERROR_INVAL *)
   - eapply asn_strtoimax_lim_ASN_STRTOX_EXPECT_MORE_correct.
 Admitted.
