src/strtoimax/sandbox.v
@@ -1,0 +1,54 @@
+eapply exec_loop.
+      eassumption.
+      eapply Heqo0.
+      eassumption.
+      exists ((_value <~ Vlong (cast_int_long Signed (Int.repr 0)))
+           ((_t'5 <~ Vptr fin_b fin_ofs)
+              ((_str <~
+                     Vptr str_b
+                     (str_ofs + Ptrofs.repr (sizeof ge tschar) * ptrofs_of_int Signed (Int.repr 1))%ptrofs)
+                 ((_sign <~ Vint ( (Int.repr 1)))
+                    ((_last_digit_max <~
+                                      Vlong
+                                      (Int64.modu
+                                         (Int64.not (cast_int_long Signed (Int.repr 0)) >>
+                                                  Int64.repr (Int.unsigned (Int.repr 1)))
+                                         (cast_int_long Signed (Int.repr 10)) +
+                                       cast_int_long Signed (Int.repr 1)))
+                       ((_t'4 <~ Vint minus_char)
+                          ((_t'6 <~ Vptr fin_b fin_ofs)
+                             ((_last_digit_max <~
+                                               Vlong
+                                               (Int64.modu
+                                                  (Int64.not (cast_int_long Signed (Int.repr 0)) >>
+                                                           Int64.repr (Int.unsigned (Int.repr 1)))
+                                                  (cast_int_long Signed (Int.repr 10))))
+                                ((_upper_boundary <~
+                                                  Vlong
+                                                  (Int64.divu
+                                                     (Int64.not (cast_int_long Signed (Int.repr 0)) >>
+                                                              Int64.repr (Int.unsigned (Int.repr 1)))
+                                                     (cast_int_long Signed (Int.repr 10))))
+                                   ((_sign <~ Vint (Int.repr 1)) le)))))))))).
+      eapply asn_strtoimax_lim_loop_ASN_STRTOX_ERROR_RANGE_correct.
+      unfold vptr.
+      all: repeat env_assumption.
+      all: repeat env_assumption.
+      repeat econstructor.
+      econstructor.
+      econstructor.
+      econstructor.
+      econstructor.
+      replace (Ptrofs.repr (sizeof ge tschar) * ptrofs_of_int Signed (Int.repr 1))%ptrofs with 1%ptrofs.
+      replace (cast_int_long Signed (Int.repr 0)) with  0%int64.
+      instantiate (4 := Unsigned).
+      simpl.
+      replace (distance (str_b, (str_ofs + 1)%ptrofs) (b, i)) with  (distance (str_b, str_ofs) (b, i) - 1)%nat.
+      eassumption.
+      unfold distance.
+      simpl.
+      admit.
+      simpl.
+      auto with ints.
+      simpl.
+      auto with ptrofs.
