src/strtoimax/switch_statements.v
@@ -1,0 +1,404 @@
+From Coq Require Import String List ZArith Psatz.
+From compcert Require Import Coqlib Integers Floats AST Ctypes Cop Clight Clightdefs Memory Values ClightBigstep Events Maps.
+Import ListNotations.
+Require Import StructTact.StructTactics.
+Require Import IntNotations asn_strtoimax_lim IntLemmas Tactics asn_strtoimax_lim_spec.
+Local Open Scope Int64Scope.
+
+(* Dealing with the switch statement *)
+Definition switch s1 s2 :=  (Sswitch (Ederef (Etempvar _str (tptr tschar)) tschar)
+                      (LScons (Some 48)
+                        Sskip
+                        (LScons (Some 49)
+                          Sskip
+                          (LScons (Some 50)
+                            Sskip
+                            (LScons (Some 51)
+                              Sskip
+                              (LScons (Some 52)
+                                Sskip
+                                (LScons (Some 53)
+                                  Sskip
+                                  (LScons (Some 54)
+                                    Sskip
+                                    (LScons (Some 55)
+                                      Sskip
+                                      (LScons (Some 56)
+                                        Sskip
+                                        (LScons (Some 57)
+                                         s1 (LScons None
+                                            s2
+                                            LSnil)))))))))))).
+
+(* If reading i a digit then we enter the correct branch and continue *)
+Lemma switch_correct_continue : forall i s1 s2 le b ofs,
+    Mem.loadv Mintx8signed m (Vptr b ofs) = Some (Vint i) ->
+    le ! _str = Some (Vptr b ofs) ->
+    is_digit i = true ->
+    forall le', (exists t, exec_stmt ge e le m s1 t le' m Out_continue) ->
+    (exists t, exec_stmt ge e le m (switch s1 s2) t le' m Out_continue).
+Proof.
+  intros.
+  cbn in H1.
+  break_exists.
+  repeat destruct_orb_hyp.
+  11: congruence.
+  all: assert (outcome_switch Out_continue = Out_continue) as Out by (simpl; auto); rewrite <- Out; repeat eexists; try reflexivity; repeat econstructor; try eassumption; try econstructor; (switch_destruct i).
+  1-9: eapply exec_Sseq_1; repeat (choose_seq s1); try (exec_Axiom || eassumption || discriminate).
+   eapply exec_Sseq_2. try (eassumption || econstructor || discriminate).
+   discriminate.
+Qed.
+
+(* If reading i a digit then we enter the correct branch and continue *)
+Lemma switch_default_correct : forall i 
+                       s1 s2 le b ofs out,
+    Mem.loadv Mint8signed m (Vptr b ofs) = Some (Vint i) ->
+    le ! _str = Some (Vptr b ofs) ->
+    is_digit i = false ->
+    forall le' m', (exists t, exec_stmt ge e le m s2 t le' m' (Out_return out)) ->
+                (exists t, exec_stmt ge e le m (switch s1 s2) t le' m' (Out_return out)).
+Proof.
+  intros until out; intros Mem Str Dig le' m' S2.
+  destruct S2 as [t S2].
+  repeat eexists.
+  replace (Out_return out) with (outcome_switch (Out_return out)) by (reflexivity).
+  econstructor.
+  repeat econstructor; try eassumption.
+  econstructor.
+  cbn in Dig.
+  repeat destruct_orb_hyp.
+  repeat (switch_destruct i).
+  try (rewrite Int.unsigned_repr in *).
+  unfold select_switch.
+  unfold select_switch_default.
+  unfold select_switch_case.
+  repeat break_if.
+  all: try congruence.
+  eapply exec_Sseq_2.
+  eassumption.
+  discriminate.
+  all: cbn;  try lia.
+       Qed.
+
+       
+
+Definition switch_1 := (Sswitch (Ederef (Etempvar _str (tptr tschar)) tschar)
+              (LScons (Some 45)
+                (Ssequence
+                  (Sset _last_digit_max
+                    (Ebinop Oadd (Etempvar _last_digit_max tlong)
+                      (Econst_int (Int.repr 1) tint) tlong))
+                  (Sset _sign
+                    (Eunop Oneg (Econst_int (Int.repr 1) tint) tint)))
+                (LScons (Some 43)
+                  (Ssequence
+                    (Sset _str
+                      (Ebinop Oadd (Etempvar _str (tptr tschar))
+                        (Econst_int (Int.repr 1) tint) (tptr tschar)))
+                    (Ssequence
+                      (Sset _t'5
+                        (Ederef (Etempvar _end (tptr (tptr tschar)))
+                          (tptr tschar)))
+                      (Sifthenelse (Ebinop Oge (Etempvar _str (tptr tschar))
+                                     (Etempvar _t'5 (tptr tschar)) tint)
+                        (Ssequence
+                          (Sassign
+                            (Ederef (Etempvar _end (tptr (tptr tschar)))
+                              (tptr tschar)) (Etempvar _str (tptr tschar)))
+                          (Sreturn (Some (Econst_int (Int.repr (-1)) tint))))
+                        Sskip)))
+                  LSnil))).
+
+Lemma switch_default_correct_1 : forall i le b ofs,
+    Mem.loadv Mint8signed m (Vptr b ofs) = Some (Vint i) ->
+    le ! _str = Some (Vptr b ofs) ->
+    (i == minus_char)%int = false ->
+    (i == plus_char)%int = false ->
+                (exists t, exec_stmt ge e le m switch_1 t le m Out_normal).
+Proof.
+  intros until ofs; intros Mem Str Min Plus.
+  repeat eexists.
+  replace (Out_normal) with (outcome_switch (Out_normal)) by (reflexivity).
+  econstructor.
+  repeat econstructor; try eassumption.
+  econstructor.
+  repeat (switch_destruct i).
+  try (rewrite Int.unsigned_repr in *).
+  unfold select_switch.
+  unfold select_switch_default.
+  unfold select_switch_case.
+  repeat break_if.
+  all: try congruence.
+  econstructor.
+  all: cbn;  try lia.
+Qed.     
+
+Lemma switch_correct_return : forall i s1 s2 le b ofs out,
+    Mem.loadv Mint8signed m (Vptr b ofs) = Some (Vint i) ->
+    le ! _str = Some (Vptr b ofs) ->
+    is_digit i = true ->
+    forall le' m', (exists t, exec_stmt ge e le m s1 t le' m' (Out_return out)) ->
+    (exists t, exec_stmt ge e le m (switch s1 s2) t le' m' (Out_return out)).
+Proof.
+  intros.
+  cbn in H1.
+  break_exists.
+  repeat destruct_orb_hyp.
+  11: congruence.
+  all: assert (outcome_switch (Out_return out) = (Out_return out)) as Out by (simpl; auto); rewrite <- Out; repeat eexists; try reflexivity; repeat econstructor; try eassumption; try econstructor; (switch_destruct i).
+  1-9: eapply exec_Sseq_1; repeat (choose_seq s1); try (exec_Axiom || eassumption || discriminate).
+   eapply exec_Sseq_2. try (eassumption || econstructor || discriminate).
+   discriminate.
+Qed.
+
+Lemma exec_loop_minus : forall le b ofs str_b str_ofs fin_b fin_ofs intp_b intp_ofs i out s1 s2,
+    le!_str = Some (Vptr str_b str_ofs)  ->
+    le!_end = Some (Vptr fin_b fin_ofs) ->
+    le!_intp = Some (Vptr intp_b intp_ofs)  ->
+    le ! _upper_boundary = Some (Vlong upper_boundary) ->
+    le ! _sign = Some (Vint (Int.repr 1)) ->
+    
+    load_addr Mptr m (fin_b, fin_ofs) = Some (Vptr b ofs) ->
+    addr_ge (str_b, str_ofs) (b, ofs) = Some false ->
+    load_addr Mint8signed m (str_b, str_ofs) = Some (Vint i) ->
+    
+    (i == minus_char)%int = true ->
+    
+    forall m', (exists t le', exec_stmt ge e
+                              ((_value <~ Vlong 0%int64)
+                                 ((_t'5 <~ Vptr b ofs)
+                                    ((_str <~ Vptr str_b (str_ofs + 1)%ptrofs)
+                                       ((_sign <~ Vint (Int.neg (Int.repr 1)))
+                                          ((_last_digit_max <~ Vlong last_digit_max_minus)
+                                             ((_t'4 <~ Vint minus_char)
+                                                ((_t'6 <~ Vptr b ofs)
+                                                   ((_last_digit_max <~ Vlong last_digit_max)
+                                                      ((_upper_boundary <~ Vlong upper_boundary)
+                                                         ((_sign <~ Vint (Int.repr 1)) le))))))))))
+                              m s1 t le' m' (Out_return out)) ->
+        exists t le', exec_stmt ge e le m (pre_loop s1 s2) t le' m' (Out_return out).
+Proof.
+  intros until s2.
+  intros Str End Intp UB Sign LA AG LA' Char m' S1.
+  break_exists.
+  unfold pre_loop.
+  repeat eexists.
+  econstructor.
+  repeat econstructor.
+  econstructor.
+  repeat econstructor.
+  econstructor.
+  repeat econstructor.
+  econstructor.
+  repeat econstructor.
+  forward.
+  unfold load_addr in *.
+  eassumption.
+  repeat env_assumption.
+  env_assumption.
+  econstructor.
+  repeat econstructor.
+ assert (sem_binary_operation ge Oge (Vptr str_b str_ofs) (typeof (Etempvar _str (tptr tschar)))
+                              (Vptr b ofs) (typeof (Etempvar _t'6 (tptr tschar))) m = Some Vfalse)  by admit; eassumption.
+ forward.
+ econstructor.
+ econstructor.
+ repeat econstructor.
+ repeat env_assumption.
+ eassumption.
+ replace Out_normal with (outcome_switch Out_normal).
+ econstructor.
+ repeat econstructor.
+ repeat env_assumption.
+ eassumption.
+ econstructor.
+ replace i with (minus_char) by admit.
+ econstructor.
+ repeat econstructor.
+ repeat env_assumption.
+ econstructor.
+ repeat econstructor.
+ forward.
+ simpl.
+ assert (sem_cmp Cge (Vptr str_b (str_ofs + Ptrofs.repr 1 * Ptrofs.of_ints (Int.repr 1))%ptrofs)
+                 (tptr tschar) (Vptr b ofs) (tptr tschar) m = Some Vfalse) by admit; eassumption.
+ forward.
+ econstructor.
+ reflexivity.
+ apply exec_Sseq_2.
+ econstructor.
+ repeat econstructor.
+ eapply H.
+ discriminate.
+Admitted.
+
+Lemma exec_loop_plus : forall le b ofs str_b str_ofs fin_b fin_ofs intp_b intp_ofs i out s1 s2,
+    le!_str = Some (Vptr str_b str_ofs)  ->
+    le!_end = Some (Vptr fin_b fin_ofs) ->
+    le!_intp = Some (Vptr intp_b intp_ofs)  ->
+    le ! _upper_boundary = Some (Vlong upper_boundary) ->
+    le ! _sign = Some (Vint (Int.repr 1)) ->
+    
+    load_addr Mptr m (fin_b, fin_ofs) = Some (Vptr b ofs) ->
+    addr_ge (str_b, str_ofs) (b, ofs) = Some false ->
+    load_addr Mint8signed m (str_b, str_ofs) = Some (Vint i) ->
+    
+    (i == plus_char)%int = true ->
+    
+    forall m', (exists t le', exec_stmt ge e
+                              ((_value <~ Vlong 0%int64)
+                                 ((_t'5 <~ Vptr b ofs)
+                                    ((_str <~ Vptr str_b (str_ofs + 1)%ptrofs)
+                                       ((_t'4 <~ Vint plus_char)
+                                          ((_t'6 <~ Vptr b ofs)
+                                             ((_last_digit_max <~ Vlong last_digit_max)
+                                                ((_upper_boundary <~ Vlong upper_boundary)
+                                                   ((_sign <~ Vint (Int.repr 1)) le))))))))
+                              m s1 t le' m' (Out_return out)) ->
+          exists t le', exec_stmt ge e le m (pre_loop s1 s2) t le' m' (Out_return out).
+Proof.
+  intros until s2.
+  intros Str End Intp UB Sign LA AG LA' Char m' S1.
+  break_exists.
+  unfold pre_loop.
+  repeat eexists.
+  econstructor.
+  repeat econstructor.
+  econstructor.
+  repeat econstructor.
+  econstructor.
+  repeat econstructor.
+  econstructor.
+  repeat econstructor.
+  forward.
+  unfold load_addr in *.
+  eassumption.
+  repeat env_assumption.
+  env_assumption.
+  econstructor.
+  repeat econstructor.
+  assert (sem_binary_operation ge Oge (Vptr str_b str_ofs) (typeof (Etempvar _str (tptr tschar)))
+                               (Vptr b ofs) (typeof (Etempvar _t'6 (tptr tschar))) m = Some Vfalse) by admit; eassumption.
+  forward.
+  econstructor.
+  econstructor.
+  repeat econstructor.
+  repeat env_assumption.
+  eassumption.
+  replace Out_normal with (outcome_switch Out_normal).
+  econstructor.
+  repeat econstructor.
+  repeat env_assumption.
+  eassumption.
+  econstructor.
+  replace i with (plus_char) by admit.
+  econstructor.
+  repeat econstructor.
+  repeat env_assumption.
+  econstructor.
+  repeat econstructor.
+  forward.
+  simpl.
+  assert (sem_cmp Cge (Vptr str_b (str_ofs + Ptrofs.repr 1 * Ptrofs.of_ints (Int.repr 1))%ptrofs)
+                  (tptr tschar) (Vptr b ofs) (tptr tschar) m = Some Vfalse) by admit; eassumption.
+  forward.
+  forward.
+  simpl.
+  assert (sem_cmp Cge (Vptr str_b (str_ofs + Ptrofs.repr 1 * Ptrofs.of_ints (Int.repr 1))%ptrofs)
+                  (tptr tschar) (Vptr b ofs) (tptr tschar) m = Some Vfalse) by admit; eassumption.
+  repeat econstructor.
+  econstructor.
+  econstructor.
+  reflexivity.
+  apply exec_Sseq_2.
+  econstructor.
+  repeat econstructor.
+  eapply H.
+  discriminate.
+Admitted.
+
+Lemma exec_loop_none : forall le b ofs str_b str_ofs fin_b fin_ofs intp_b intp_ofs i out s1 s2,
+    le!_str = Some (Vptr str_b str_ofs)  ->
+    le!_end = Some (Vptr fin_b fin_ofs) ->
+    le!_intp = Some (Vptr intp_b intp_ofs)  ->
+    le ! _upper_boundary = Some (Vlong upper_boundary) ->
+    le ! _sign = Some (Vint (Int.repr 1)) ->
+    
+    load_addr Mptr m (fin_b, fin_ofs) = Some (Vptr b ofs) ->
+    addr_ge (str_b, str_ofs) (b, ofs) = Some false ->
+    load_addr Mint8signed m (str_b, str_ofs) = Some (Vint i) ->
+    
+    (i == plus_char)%int = false ->
+    (i == minus_char)%int = false ->
+    
+    forall le' m', (exists t, exec_stmt ge e
+                              ((_value <~ Vlong (cast_int_long Signed (Int.repr 0)))
+       ((_t'4 <~ Vint i)
+          ((_t'6 <~ Vptr b ofs)
+             ((_last_digit_max <~
+               Vlong
+                 (Int64.modu
+                    (Int64.not (cast_int_long Signed (Int.repr 0)) >>
+                     Int64.repr (Int.unsigned (Int.repr 1))) (cast_int_long Signed (Int.repr 10))))
+                ((_upper_boundary <~
+                  Vlong
+                    (Int64.divu
+                       (Int64.not (cast_int_long Signed (Int.repr 0)) >>
+                        Int64.repr (Int.unsigned (Int.repr 1)))
+                       (cast_int_long Signed (Int.repr 10)))) ((_sign <~ Vint (Int.repr 1)) le))))))
+                              m s1 t le' m' (Out_return out)) ->
+          exists t, exec_stmt ge e le m (pre_loop s1 s2) t le' m' (Out_return out).
+Proof.
+  intros until s2.
+  intros Str End Intp UB Sign LA AG LA' CharP CharM le' m' S1.
+  destruct S1.
+ 
+  unfold pre_loop.
+  destruct (switch_default_correct_1 i ((_t'4 <~ Vint i)
+       ((_t'6 <~ Vptr b ofs)
+          ((_last_digit_max <~
+            Vlong
+              (Int64.modu
+                 (Int64.not (cast_int_long Signed (Int.repr 0)) >>
+                  Int64.repr (Int.unsigned (Int.repr 1))) (cast_int_long Signed (Int.repr 10))))
+             ((_upper_boundary <~
+               Vlong
+                 (Int64.divu
+                    (Int64.not (cast_int_long Signed (Int.repr 0)) >>
+                     Int64.repr (Int.unsigned (Int.repr 1))) (cast_int_long Signed (Int.repr 10))))
+                ((_sign <~ Vint (Int.repr 1)) le))))) str_b str_ofs).
+  all: try eassumption; env_assumption.
+  
+  repeat env_assumption.
+  repeat eexists.
+  econstructor.
+  repeat econstructor.
+  econstructor.
+  repeat econstructor.
+  econstructor.
+  repeat econstructor.
+  econstructor.
+  repeat econstructor.
+  forward.
+  unfold load_addr in *.
+  eassumption.
+  repeat env_assumption.
+  env_assumption.
+  econstructor.
+  repeat econstructor.
+  assert (sem_binary_operation ge Oge (Vptr str_b str_ofs) (typeof (Etempvar _str (tptr tschar)))
+                               (Vptr b ofs) (typeof (Etempvar _t'6 (tptr tschar))) m = Some Vfalse) by admit; eassumption.
+  forward.
+  econstructor.
+  econstructor.
+  repeat econstructor.
+  repeat env_assumption.
+  eassumption.
+  eassumption.
+  apply exec_Sseq_2.
+  econstructor.
+  repeat econstructor.
+  clear H0.
+  eassumption.
+  congruence.
+Admitted.
